CollapsingTowers/TwoLevelBasic/Defs.lean
@@ -4,3 +4,4 @@ import CollapsingTowers.TwoLevelBasic.OperationalSemantics.Defs
 import CollapsingTowers.TwoLevelBasic.SyntacticTyping.Defs
 import CollapsingTowers.TwoLevelBasic.SyntacticSoundness.Defs
 import CollapsingTowers.TwoLevelBasic.CtxEquiv.Defs
+import CollapsingTowers.TwoLevelBasic.LogicalEquiv.Defs
