CollapsingTowers/TwoLevelBasic/LogicalEquiv/Defs.lean
@@ -1,0 +1,1 @@
+import CollapsingTowers.TwoLevelBasic.LogicalEquiv.LogicalRelation
