CollapsingTowers/TwoLevelBasic/LogicalEquiv/LogicalRelation.lean
@@ -1,0 +1,216 @@
+import CollapsingTowers.TwoLevelBasic.SyntacticSoundness.Defs
+import CollapsingTowers.TwoLevelBasic.OperationalSemantics.Defs
+
+mutual
+@[simp]
+def log_equiv_value : Expr → Expr → Ty → Prop
+  --
+  --
+  -- 𝓥⟦ℕ⟧ ≜ {(n, n) | n ∈ ℕ}
+  | .lit n₀, .lit n₁, .nat => n₀ = n₁
+  --
+  --
+  -- 𝓥⟦τ𝕒 → τ𝕓⟧ ≜ {
+  --   (λx.e₀, λx.e₁) |
+  --   ⦰ ⊢ λx.e₀ : τ𝕒 → τ𝕓 ∧
+  --   ⦰ ⊢ λx.e₁ : τ𝕒 → τ𝕓 ∧
+  --   ∀ (v₀, v₁) ∈ 𝓥⟦τ𝕒⟧. (λx.e₀ @ v₀, λx.e₁ @ v₁) ∈ 𝓔⟦τ𝕓⟧
+  -- }
+  | .lam e₀, .lam e₁, (.arrow τ𝕒 τ𝕓 ⊥) =>
+    typing ⦰ 𝟚 (.lam e₀) (.arrow τ𝕒 τ𝕓 ⊥) ⊥ ∧
+    typing ⦰ 𝟚 (.lam e₁) (.arrow τ𝕒 τ𝕓 ⊥) ⊥ ∧
+    ∀ v₀ v₁,
+      log_equiv_value v₀ v₁ τ𝕒 →
+      log_equiv_expr (.app₁ (.lam e₀) v₀) (.app₁ (.lam e₁) v₁) τ𝕓
+  | _, _, _ => false
+
+-- 𝓔⟦τ⟧ₖ ≜ {(e₀, e₁) | ∃ v₀ v₁. e₀ ⇾* v₀ ∧ e₁ ⇾* v₁ ∧ (v₀, v₁) ∈ 𝓥⟦τ⟧}
+@[simp]
+def log_equiv_expr (e₀ : Expr) (e₁ : Expr) (τ : Ty) : Prop :=
+  ∃ v₀ v₁,
+    (e₀ ⇝* v₀) ∧ (e₁ ⇝* v₁) ∧ log_equiv_value v₀ v₁ τ
+end
+
+inductive typing.subst : Subst → TEnv → Prop where
+  | nil : typing.subst [] ⦰
+  | cons : ∀ v γ τ Γ,
+    value v →
+    typing ⦰ 𝟚 v τ ⊥ →
+    typing.subst γ Γ →
+    typing.subst (v :: γ) ((τ, 𝟚) :: Γ)
+
+inductive log_equiv_env : Subst → Subst → TEnv → Prop where
+  | nil : log_equiv_env [] [] ⦰
+  | cons : ∀ v₀ γ₀ v₁ γ₁ τ Γ,
+    log_equiv_value v₀ v₁ τ →
+    log_equiv_env γ₀ γ₁ Γ →
+    log_equiv_env (v₀ :: γ₀) (v₁ :: γ₁) ((τ, 𝟚) :: Γ)
+
+-- Γ ⊧ e₀ ≈𝑙𝑜𝑔 e₁ : τ ≜
+--   Γ ⊢ e₀ : τ ∧
+--   Γ ⊢ e₁ : τ ∧
+--   ∀ (γ₀, γ₁) ∈ 𝓖⟦Γ⟧. (γ₀(e₀), γ₁(e₁)) ∈ 𝓔⟦τ⟧
+@[simp]
+def log_equiv (Γ : TEnv) (e₀ : Expr) (e₁ : Expr) (τ : Ty) : Prop :=
+  typing Γ 𝟚 e₀ τ ⊥ ∧
+  typing Γ 𝟚 e₁ τ ⊥ ∧
+  ∀ γ₀ γ₁,
+    log_equiv_env γ₀ γ₁ Γ →
+    log_equiv_expr (msubst γ₀ e₀) (msubst γ₁ e₁) τ
+
+lemma log_equiv_value.syntactic.value :
+  ∀ v₀ v₁ τ,
+    log_equiv_value v₀ v₁ τ →
+    value v₀ ∧ value v₁ :=
+  by
+  intros v₀ v₁ τ Hsem_value
+  cases τ
+  case nat =>
+    cases v₀ <;> cases v₁ <;> simp at Hsem_value
+    constructor
+    apply value.lit
+    apply value.lit
+  case arrow φ =>
+    cases v₀ <;> cases v₁ <;> cases φ <;> simp at Hsem_value
+    have ⟨Hτ₀, Hτ₁, _⟩ := Hsem_value
+    constructor
+    apply value.lam; apply typing.regular _ _ _ _ _ Hτ₀
+    apply value.lam; apply typing.regular _ _ _ _ _ Hτ₁
+  all_goals simp at Hsem_value
+
+lemma log_equiv_value.syntactic.typing :
+  ∀ v₀ v₁ τ,
+    log_equiv_value v₀ v₁ τ →
+    typing ⦰ 𝟚 v₀ τ ⊥ ∧ typing ⦰ 𝟚 v₁ τ ⊥ :=
+  by
+  intros v₀ v₁ τ Hsem_value
+  cases τ
+  case nat =>
+    cases v₀ <;> cases v₁ <;> simp at Hsem_value
+    constructor; apply typing.lit; apply typing.lit
+  case arrow φ =>
+    cases v₀ <;> cases v₁ <;> cases φ <;> simp at Hsem_value
+    have ⟨Hτ₀, Hτ₁, _⟩ := Hsem_value
+    constructor; apply Hτ₀; apply Hτ₁
+  all_goals simp at Hsem_value
+
+lemma log_equiv_value.apply :
+  ∀ f₀ arg₀ f₁ arg₁ τ𝕒 τ𝕓,
+    log_equiv_value f₀ f₁ (.arrow τ𝕒 τ𝕓 ⊥) →
+    log_equiv_value arg₀ arg₁ τ𝕒 →
+    log_equiv_expr (.app₁ f₀ arg₀) (.app₁ f₁ arg₁) τ𝕓 :=
+  by
+  intros f₀ arg₀ f₁ arg₁ τ𝕒 τ𝕓 Hsem_value_fun Hsem_value_arg
+  cases f₀ <;> cases f₁ <;> simp only [log_equiv_value] at Hsem_value_fun <;> try contradiction
+  have ⟨_, _, Hsem_value_fun⟩ := Hsem_value_fun
+  apply Hsem_value_fun; apply Hsem_value_arg
+
+lemma log_equiv_env.length :
+  ∀ γ₀ γ₁ Γ,
+    log_equiv_env γ₀ γ₁ Γ →
+    γ₀.length = Γ.length ∧
+    γ₁.length = Γ.length :=
+  by
+  intros γ₀ γ₁ Γ H
+  induction H
+  case nil => simp
+  case cons IH =>
+    constructor
+    . simp; apply IH.left
+    . simp; apply IH.right
+
+lemma log_equiv_env.binds_log_equiv_value :
+  ∀ γ₀ γ₁ Γ x τ,
+    log_equiv_env γ₀ γ₁ Γ →
+    binds x (τ, 𝟚) Γ →
+    log_equiv_value (msubst γ₀ (.fvar x)) (msubst γ₁ (.fvar x)) τ :=
+  by
+  intros γ₀ γ₁ Γ x τ HsemΓ Hbinds
+  induction HsemΓ
+  case nil => nomatch Hbinds
+  case cons v₀ γ₀ v₁ γ₁ τ Γ Hsem_value HsemΓ IH =>
+    have ⟨Hτ₀, Hτ₁⟩ := log_equiv_value.syntactic.typing _ _ _ Hsem_value
+    have ⟨HEq₀, HEq₁⟩ := log_equiv_env.length _ _ _ HsemΓ
+    simp [HEq₀, HEq₁]
+    by_cases HEqx : Γ.length = x
+    . simp [if_pos HEqx]
+      simp [if_pos HEqx] at Hbinds
+      rw [← Hbinds, identity.msubst, identity.msubst]
+      apply Hsem_value
+      apply typing.closed_at_env _ _ _ _ _ Hτ₁
+      apply typing.closed_at_env _ _ _ _ _ Hτ₀
+    . simp [if_neg HEqx]
+      simp [if_neg HEqx] at Hbinds
+      apply IH; apply Hbinds
+
+lemma log_equiv_env.mwf :
+  ∀ γ₀ γ₁ Γ,
+    log_equiv_env γ₀ γ₁ Γ →
+    mwf γ₀ ∧ mwf γ₁ :=
+  by
+  intros γ₀ γ₁ Γ HsemΓ
+  induction HsemΓ
+  case nil => repeat constructor
+  case cons Hsem_value _ IH =>
+    have ⟨Hτ₀, Hτ₁⟩ := log_equiv_value.syntactic.typing _ _ _ Hsem_value
+    constructor
+    . constructor
+      apply typing.wf _ _ _ _ _ Hτ₀
+      apply IH.left
+    . constructor
+      apply typing.wf _ _ _ _ _ Hτ₁
+      apply IH.right
+
+lemma log_equiv_env.msubst.typing :
+  ∀ γ₀ γ₁ e₀ e₁ Γ τ,
+    typing Γ 𝟚 e₀ τ ⊥ →
+    typing Γ 𝟚 e₁ τ ⊥ →
+    log_equiv_env γ₀ γ₁ Γ →
+    typing ⦰ 𝟚 (msubst γ₀ e₀) τ ⊥ ∧
+    typing ⦰ 𝟚 (msubst γ₁ e₁) τ ⊥ :=
+  by
+  intros γ₀ γ₁ e₀ e₁ Γ τ Hτ₀ Hτ₁ HsemΓ
+  induction HsemΓ generalizing e₀ e₁
+  case nil => constructor; apply Hτ₀; apply Hτ₁
+  case cons Γ Hsem_value HsemΓ IH =>
+    have ⟨HEq₀, HEq₁⟩ := log_equiv_env.length _ _ _ HsemΓ
+    have ⟨Hτv₀, Hτv₁⟩ := log_equiv_value.syntactic.typing _ _ _ Hsem_value
+    apply IH
+    . rw [HEq₀]; apply preservation.dynamic_subst; rw [← List.append_nil Γ]
+      apply typing.weakening; apply Hτv₀; apply Hτ₀
+    . rw [HEq₁]; apply preservation.dynamic_subst; rw [← List.append_nil Γ]
+      apply typing.weakening; apply Hτv₁; apply Hτ₁
+
+lemma log_equiv_env.syntactic.typing :
+  ∀ γ₀ γ₁ Γ,
+    log_equiv_env γ₀ γ₁ Γ →
+    typing.subst γ₀ Γ ∧
+    typing.subst γ₁ Γ :=
+  by
+  intros γ₀ γ₁ Γ HsemΓ
+  induction HsemΓ
+  case nil =>
+    constructor
+    . apply typing.subst.nil
+    . apply typing.subst.nil
+  case cons Hsem_value _ IH =>
+    have ⟨IH₀, IH₁⟩ := IH
+    have ⟨Hτv₀, Hτv₁⟩ := log_equiv_value.syntactic.typing _ _ _ Hsem_value
+    have ⟨Hvalue₀, Hvalue₁⟩ := log_equiv_value.syntactic.value _ _ _ Hsem_value
+    constructor
+    . apply typing.subst.cons
+      apply Hvalue₀; apply Hτv₀
+      apply IH₀
+    . apply typing.subst.cons
+      apply Hvalue₁; apply Hτv₁
+      apply IH₁
+
+lemma typing.subst.length :
+  ∀ γ Γ,
+    typing.subst γ Γ →
+    γ.length = Γ.length :=
+  by
+  intros γ Γ Hτγ
+  induction Hτγ
+  case nil => simp
+  case cons IH => simp [IH]
